Unrestriction.thy
@@ -27,6 +27,11 @@ lemma unrest_var_union [unrest]:
   by (simp add: expr_defs lens_defs)
      (metis scene_override_union scene_override_unit scene_union_incompat)
 
+lemma unrest_neg_union:
+  assumes "A ##\<^sub>S B" "- A \<sharp> P" "- B \<sharp> P"
+  shows "(- (A ; B)) \<sharp> P"
+  using assms by (simp add: unrest_def scene_override_commute scene_override_union)
+
 lemma unrest_subscene: "\<lbrakk> idem_scene a; a \<sharp> e; b \<subseteq>\<^sub>S a \<rbrakk> \<Longrightarrow> b \<sharp> e"
   by (metis (mono_tags, hide_lams) subscene_eliminate unrest_def)
 
@@ -37,19 +42,44 @@ lemma unrest_lens_comp [unrest]: "\<lbrakk> vwb_lens x; vwb_lens y; $x \<sharp> 
 lemma unrest_lit [unrest]: "x \<sharp> \<guillemotleft>v\<guillemotright>"
   by (simp add: expr_defs)
 
-lemma unrest_var [unrest]:
+lemma unrest_var [unrest]: 
+  "\<lbrakk> vwb_lens x; idem_scene a; var_alpha x \<bowtie>\<^sub>S a \<rbrakk> \<Longrightarrow> a \<sharp> $x"
+  by (auto simp add: unrest_def scene_indep_override var_alpha_def)
+     (metis lens_override_def lens_override_idem lens_scene_override mwb_lens_weak vwb_lens_mwb weak_lens_def)
+
+lemma unrest_var': 
+  "x \<notin>\<^sub>S a \<Longrightarrow> a \<sharp> $x"
+  by (simp add: unrest_def)
+
+lemma unrest_var_single [unrest]:
   "\<lbrakk> mwb_lens x; x \<bowtie> y \<rbrakk> \<Longrightarrow> $x \<sharp> $y"
   by (simp add: expr_defs lens_indep.lens_put_irr2 lens_indep_sym lens_override_def lens_scene_override var_alpha_def)
 
-lemma unrest_uop [unrest]:
+lemma unrest_conj [unrest]:
+  "\<lbrakk> x \<sharp> P; x \<sharp> Q \<rbrakk> \<Longrightarrow> x \<sharp> (P \<and> Q)"
+  by (auto simp add: expr_defs)
+
+lemma unrest_not [unrest]:
+  "\<lbrakk> x \<sharp> P \<rbrakk> \<Longrightarrow> x \<sharp> (\<not> P)"
+  by (auto simp add: expr_defs)
+
+lemma unrest_disj [unrest]:
+  "\<lbrakk> x \<sharp> P; x \<sharp> Q \<rbrakk> \<Longrightarrow> x \<sharp> (P \<or> Q)"
+  by (auto simp add: expr_defs)
+
+lemma unrest_implies [unrest]:
+  "\<lbrakk> x \<sharp> P; x \<sharp> Q \<rbrakk> \<Longrightarrow> x \<sharp> (P \<longrightarrow> Q)"
+  by (auto simp add: expr_defs)
+
+lemma unrest_uop:
   "\<lbrakk> x \<sharp> e \<rbrakk> \<Longrightarrow> x \<sharp> \<guillemotleft>f\<guillemotright> e"
   by (auto simp add: expr_defs)
 
-lemma unrest_bop [unrest]:
+lemma unrest_bop:
   "\<lbrakk> x \<sharp> e\<^sub>1; x \<sharp> e\<^sub>2 \<rbrakk> \<Longrightarrow> x \<sharp> \<guillemotleft>f\<guillemotright> e\<^sub>1 e\<^sub>2"
   by (auto simp add: expr_defs)
 
-lemma unrest_trop [unrest]:
+lemma unrest_trop:
   "\<lbrakk> x \<sharp> e\<^sub>1; x \<sharp> e\<^sub>2; x \<sharp> e\<^sub>3 \<rbrakk> \<Longrightarrow> x \<sharp> \<guillemotleft>f\<guillemotright> e\<^sub>1 e\<^sub>2 e\<^sub>3"
   by (auto simp add: expr_defs)
 
